deps/coq-poulet4/lib/V1Model.v
@@ -1,0 +1,69 @@
+Require Import Strings.String.
+Require Import Coq.Bool.Bool.
+Require Import Coq.ZArith.BinInt.
+Require Import Coq.ZArith.ZArith.
+Require Import Coq.Lists.List.
+Require Import Coq.Program.Program.
+Require Import Typed.
+Require Import Syntax.
+Require Import P4Int.
+Require Import Target.
+Require Import Maps.
+Import ListNotations.
+
+Section V1Model.
+
+Context {tags_t: Type}.
+Context {Expression: Type}.
+Notation ident := (P4String.t tags_t).
+Notation path := (list ident).
+Notation Val := (@ValueBase tags_t).
+Notation table_entry := (@table_entry tags_t Expression).
+Notation action_ref := (@action_ref tags_t Expression).
+
+Inductive register := mk_register {
+  reg_size : Z;
+  reg_content : list bool
+}.
+
+Definition new_register (size : Z) :=
+  mk_register size (repeat false (Z.to_nat size)).
+
+Definition extern_state := @PathMap.t tags_t register.
+
+Definition extern_empty : extern_state := PathMap.empty.
+
+Axiom dummy_tag : tags_t.
+Definition register_string : ident := {| P4String.tags := dummy_tag; P4String.str := "register" |}.
+
+Definition alloc_extern (s : extern_state) (class : ident) (p : path) (args : list Val) :=
+  if P4String.equivb class register_string then
+    match args with
+    | [ValBaseInteger size]
+    | [ValBaseBit _ size]
+    | [ValBaseInt _ size] =>
+        PathMap.set p (new_register size) s
+    | _ => s
+    end
+  else
+    s.
+
+Axiom exec_extern : extern_state -> ident (* class *) -> ident (* method *) -> path -> list Val -> extern_state -> list Val -> option Val -> Prop.
+
+Axiom extern_get_entries : extern_state -> path -> list table_entry.
+
+Axiom extern_match : list (Val * ident) -> list table_entry -> option action_ref.
+
+Instance V1ModelExternSem : ExternSem := Build_ExternSem
+  extern_state
+  extern_empty
+  alloc_extern
+  exec_extern
+  extern_get_entries
+  extern_match.
+
+Axiom exec_prog : (path -> extern_state -> list Val -> extern_state -> list Val -> Prop) -> Prop.
+
+Instance V1Model : Target := Build_Target _ exec_prog.
+
+End V1Model.
